experiments/state_on_io/MST.Repr.fst
@@ -6,10 +6,8 @@ open FStar.Calc
 open FStar.Preorder
 open FStar.Monotonic.Heap
 open FStar.Ghost
-open FStar.Universe
 
 open Free
-open DMFree
 open GuardedDMFree
 
 module L = FStar.List.Tot.Base
@@ -80,16 +78,12 @@ type mst_cmds : Type0 -> Type u#1 =
 
 (* CGetHeap cannot be part of mst_cmds because erased heap : Type u#1 (not
    Type0): heap lives at universe 1 because it stores values of arbitrary
-   Type0 types. Thus it gets its own command type, indexed at universe 1.
-   (The u#2 is padding: cmd_sum at index universe 1 lives at u#2, and both
-   its summands must live there too.) *)
+   Type0 types. Thus it gets its own command type, indexed at universe 1,
+   which goes on the second channel of the free monad (whose index universe
+   is independent of the first channel's). *)
 noeq
-type heap_cmds : Type u#1 -> Type u#2 =
+type heap_cmds : Type u#1 -> Type u#1 =
 | CGetHeap : heap_cmds (erased heap)
-
-(** Combined MST commands: mst_cmds is lifted to index universe 1
-    (via cmd_downgrade) so that it can be summed with heap_cmds. *)
-let mst_all_cmds : Type u#1 -> Type u#2 = cmd_sum (cmd_downgrade u#1 u#1 mst_cmds) heap_cmds
 
 (** ** END Section 2: MST commands **)
 
@@ -216,12 +210,6 @@ let heap_cwp (_c:caller) (#r:Type u#1) (op:heap_cmds r) : hist #mst_event r =
        coercion inserted by the elaborator *)
     | CGetHeap -> p [] (coerce_eq () (hide (current_heap h)))
 
-(** Command WPs for the combined commands: the WPs of the downgraded
-    mst_cmds + the WPs of heap_cmds. *)
-unfold
-let mst_all_cwp : cmd_wp mst_all_cmds mst_event =
-  cmd_wp_sum (cmd_wp_downgrade mst_cwp) heap_cwp
-
 (** Lifting from hist-based WPs to state-based WPs.
     Converts a hist WP over mst_event events to a state-based WP.
     apply_events folds the local trace from h0 to compute the final heap. **)
@@ -250,10 +238,10 @@ let embed_st_to_hist (#a:Type) (wp:st_mwp_h heap a) : hist #mst_event a =
     Internally a dm tree (free monad + theta refinement) whose hist WP
     is the embedding of the state-based WP via embed_st_to_hist. *)
 let mst (a:Type) (wp:st_mwp_h heap a) =
-  gdm mst_all_cmds mst_event mst_all_cwp a (embed_st_to_hist wp)
+  gdm mst_cmds heap_cmds mst_event mst_cwp heap_cwp a (embed_st_to_hist wp)
 
 let mst_return (#a:Type) (x:a) : mst a (st_return x) =
-  gdm_subcomp mst_all_cwp (hist_return x) (embed_st_to_hist (st_return x)) (gdm_return mst_all_cwp x)
+  gdm_subcomp mst_cwp heap_cwp (hist_return x) (embed_st_to_hist (st_return x)) (gdm_return mst_cwp heap_cwp x)
 
 (** embed_st_to_hist is a lax monad morphism: it distributes over bind.
     Proof sketch: unfolding both sides yields wp_v applied to different
@@ -343,8 +331,8 @@ let mst_bind
   let hwp_v = embed_st_to_hist wp_v in
   let hwp_f = fun x -> embed_st_to_hist (wp_f x) in
   lemma_embed_bind_dist wp_v wp_f;
-  gdm_subcomp mst_all_cwp (hist_bind hwp_v hwp_f) (embed_st_to_hist (st_bind wp_v wp_f))
-    (gdm_bind mst_all_cwp hwp_v hwp_f v f)
+  gdm_subcomp mst_cwp heap_cwp (hist_bind hwp_v hwp_f) (embed_st_to_hist (st_bind wp_v wp_f))
+    (gdm_bind mst_cwp heap_cwp hwp_v hwp_f v f)
 
 let mst_subcomp
   (#a : Type)
@@ -362,38 +350,21 @@ let guard_st_wp (pre:pure_pre) : st_mwp_h heap (squash pre) =
   wp'
 
 let guard_return (pre:pure_pre) : mst (squash pre) (guard_st_wp pre) =
-  gdm_subcomp mst_all_cwp (guard_wp pre) (embed_st_to_hist (guard_st_wp pre))
-    (gdm_guard mst_all_cwp pre)
+  gdm_subcomp mst_cwp heap_cwp (guard_wp pre) (embed_st_to_hist (guard_st_wp pre))
+    (gdm_guard mst_cwp heap_cwp pre)
 
-(** Runs a Type0-resulting command through the downgrade wrapper, hiding the
-    universe raise/downgrade round-trip: the WP is the same as if the command
-    was part of the free monad directly (like gdm_cmd provides). *)
 #push-options "--z3rlimit 40"
-let mst_cmd (c:caller) (#r:Type0) (op:mst_cmds r)
-  : gdm mst_all_cmds mst_event mst_all_cwp r (hist_bind (mst_cwp c op) (fun ri -> hist_return ri)) =
-  let dop : mst_all_cmds (raise_t u#0 u#1 r) = CmdL (CmdDowngrade op) in
-  let wp_v = hist_bind (mst_all_cwp c dop) (fun ri -> hist_return ri) in
-  let wp_f : raise_t u#0 u#1 r -> hist #mst_event r =
-    fun x -> hist_return (downgrade_val x) in
-  let m = gdm_bind mst_all_cwp wp_v wp_f
-            (gdm_cmd mst_all_cwp c dop)
-            (fun x -> gdm_return mst_all_cwp (downgrade_val x)) in
-  gdm_subcomp mst_all_cwp
-    (hist_bind wp_v wp_f)
-    (hist_bind (mst_cwp c op) (fun ri -> hist_return ri))
-    m
-
 let mst_read (#a:Type) (#rel:preorder a) (r:mref a rel) : mst a (read_wp r) =
-  gdm_subcomp mst_all_cwp
+  gdm_subcomp mst_cwp heap_cwp
     (hist_bind (mst_cwp Prog (CRead r)) (fun x -> hist_return x))
     (embed_st_to_hist (read_wp r))
-    (mst_cmd Prog (CRead r))
+    (gdm_cmd1 mst_cwp heap_cwp Prog (CRead r))
 
 let mst_write (#a:Type) (#rel:preorder a) (r:mref a rel) (v:a) : mst unit (write_wp r v) =
-  gdm_subcomp mst_all_cwp
+  gdm_subcomp mst_cwp heap_cwp
     (hist_bind (mst_cwp Prog (CWrite r v)) (fun x -> hist_return x))
     (embed_st_to_hist (write_wp r v))
-    (mst_cmd Prog (CWrite r v))
+    (gdm_cmd1 mst_cwp heap_cwp Prog (CWrite r v))
 
 #push-options "--fuel 2"
 let lemma_alloc_embed (#a:Type) (#rel:preorder a) (init:a) (p:hist_post #mst_event (mref a rel)) (h:list mst_event) :
@@ -406,30 +377,30 @@ let lemma_alloc_embed (#a:Type) (#rel:preorder a) (init:a) (p:hist_post #mst_eve
 
 let mst_alloc (#a:Type) (#rel:preorder a) (init:a) : mst (mref a rel) (alloc_wp init) =
   Classical.forall_intro_2 (Classical.move_requires_2 (lemma_alloc_embed #a #rel init));
-  gdm_subcomp mst_all_cwp
+  gdm_subcomp mst_cwp heap_cwp
     (hist_bind (mst_cwp Prog (CAlloc init)) (fun x -> hist_return x))
     (embed_st_to_hist (alloc_wp init))
-    (mst_cmd Prog (CAlloc init))
+    (gdm_cmd1 mst_cwp heap_cwp Prog (CAlloc init))
 
 let mst_witness (pred:heap_predicate_stable) : mst unit (witness_wp pred) =
-  gdm_subcomp mst_all_cwp
+  gdm_subcomp mst_cwp heap_cwp
     (hist_bind (mst_cwp Prog (CWitness pred)) (fun x -> hist_return x))
     (embed_st_to_hist (witness_wp pred))
-    (mst_cmd Prog (CWitness pred))
+    (gdm_cmd1 mst_cwp heap_cwp Prog (CWitness pred))
 
 let mst_recall (pred:heap_predicate_stable) : mst unit (recall_wp pred) =
-  gdm_subcomp mst_all_cwp
+  gdm_subcomp mst_cwp heap_cwp
     (hist_bind (mst_cwp Prog (CRecall pred)) (fun x -> hist_return x))
     (embed_st_to_hist (recall_wp pred))
-    (mst_cmd Prog (CRecall pred))
+    (gdm_cmd1 mst_cwp heap_cwp Prog (CRecall pred))
 
-(** CGetHeap's result (erased heap) lives at universe 1, so the command is
-    called directly (no downgrade wrapper needed). *)
+(** CGetHeap's result (erased heap) lives at universe 1, so the command
+    goes through the second channel of the free monad. *)
 let mst_get_heap : mst (erased heap) get_heap_wp =
-  gdm_subcomp mst_all_cwp
-    (hist_bind (mst_all_cwp Prog (CmdR CGetHeap)) (fun x -> hist_return x))
+  gdm_subcomp mst_cwp heap_cwp
+    (hist_bind (heap_cwp Prog CGetHeap) (fun x -> hist_return x))
     (embed_st_to_hist get_heap_wp)
-    (gdm_cmd mst_all_cwp Prog (CmdR CGetHeap))
+    (gdm_cmd2 mst_cwp heap_cwp Prog CGetHeap)
 #pop-options
 
 (** ** END Section 4: Dijkstra Monad **)
